% Options for packages loaded elsewhere
\PassOptionsToPackage{unicode}{hyperref}
\PassOptionsToPackage{hyphens}{url}
%
\documentclass[
]{article}
\usepackage{lmodern}
\usepackage{amssymb,amsmath}
\usepackage{ifxetex,ifluatex}
\ifnum 0\ifxetex 1\fi\ifluatex 1\fi=0 % if pdftex
  \usepackage[T1]{fontenc}
  \usepackage[utf8]{inputenc}
  \usepackage{textcomp} % provide euro and other symbols
\else % if luatex or xetex
  \usepackage{unicode-math}
  \defaultfontfeatures{Scale=MatchLowercase}
  \defaultfontfeatures[\rmfamily]{Ligatures=TeX,Scale=1}
\fi
% Use upquote if available, for straight quotes in verbatim environments
\IfFileExists{upquote.sty}{\usepackage{upquote}}{}
\IfFileExists{microtype.sty}{% use microtype if available
  \usepackage[]{microtype}
  \UseMicrotypeSet[protrusion]{basicmath} % disable protrusion for tt fonts
}{}
\makeatletter
\@ifundefined{KOMAClassName}{% if non-KOMA class
  \IfFileExists{parskip.sty}{%
    \usepackage{parskip}
  }{% else
    \setlength{\parindent}{0pt}
    \setlength{\parskip}{6pt plus 2pt minus 1pt}}
}{% if KOMA class
  \KOMAoptions{parskip=half}}
\makeatother
\usepackage{xcolor}
\IfFileExists{xurl.sty}{\usepackage{xurl}}{} % add URL line breaks if available
\IfFileExists{bookmark.sty}{\usepackage{bookmark}}{\usepackage{hyperref}}
\hypersetup{
  pdftitle={A Mosquito Problem},
  pdfauthor={Chris Berg},
  hidelinks,
  pdfcreator={LaTeX via pandoc}}
\urlstyle{same} % disable monospaced font for URLs
\usepackage[margin=1in]{geometry}
\usepackage{graphicx,grffile}
\makeatletter
\def\maxwidth{\ifdim\Gin@nat@width>\linewidth\linewidth\else\Gin@nat@width\fi}
\def\maxheight{\ifdim\Gin@nat@height>\textheight\textheight\else\Gin@nat@height\fi}
\makeatother
% Scale images if necessary, so that they will not overflow the page
% margins by default, and it is still possible to overwrite the defaults
% using explicit options in \includegraphics[width, height, ...]{}
\setkeys{Gin}{width=\maxwidth,height=\maxheight,keepaspectratio}
% Set default figure placement to htbp
\makeatletter
\def\fps@figure{htbp}
\makeatother
\setlength{\emergencystretch}{3em} % prevent overfull lines
\providecommand{\tightlist}{%
  \setlength{\itemsep}{0pt}\setlength{\parskip}{0pt}}
\setcounter{secnumdepth}{-\maxdimen} % remove section numbering

\title{A Mosquito Problem}
\author{Chris Berg}
\date{4/26/2020}

\begin{document}
\maketitle

\emph{This problem was written by George Evans and comes from the
University of Oregon core macroeconomics exam, in July of 2013.}

\hypertarget{setup}{%
\subsection{Setup}\label{setup}}

Imagine that at time \(t\) there are \(M_t > 0\) mosquitos carrying a
deadly novel influenza virus around an economy with labor force
\(L_t > 0\). We are given the following equations of reproduction for
the labor force, and the mosquito population:

\begin{align}

\dot{M} &= (\phi - \sigma)M_t - Z_t \\
\dot{L} &= nL_t - \phi M_t

\end{align}

Here, \(\phi > 0\) is the growth rate of the virulent mosquito
population and \(\sigma > 0\) is the mortality rate of the mosquitos (at
least, the ones with the virus). The labor force grows at rate
\(n > 0\). \(Z_t > 0\) can be thought of, in general, as a good which
abates the mosquitos who have the virus (i.e.~mosquito repellant, or
even as general as the disposal of food which the mosquitos feast upon).
The abatement good and the consumption good \(C_t > 0\) can each be
produced using a production technology with unit labor requirements
\(a,b > 0\) \footnote{The careful observer will notice this equation is
  actually the production possibilities frontier for a given labor
  force.}:

\begin{align}

aZ_t + bC_t = L_t

\end{align}

We can take initial values \(M(0) , L(0)\) as given.

\hypertarget{task-a}{%
\subsection{Task A}\label{task-a}}

\begin{enumerate}
\def\labelenumi{\arabic{enumi}.}
\tightlist
\item
  \emph{Show, for a suitable constant \(k\) depending on the parameters,
  that if \(x = \frac{L}{M}\) and \(z = \frac{Z}{M}\)\ldots{}}
\end{enumerate}

\[ \dot{x} = (z-k)x - \phi \]

\textbf{Answer:}

Start off by noticing that given the definition of \(x\), we can write
\[\dot{x} \equiv \frac{dx}{dt} =  \frac{dLM^{-1}}{dt} = \frac{\dot{L}M - L\dot{M}}{M^2} \]

Breaking the difference apart and substituting yields \begin{align} 

\dot{x} &= \frac{nL - \phi M}{M} - \frac{L}{M}((\phi - \sigma) - z) \\
        &= nx - (\phi - \sigma)x + zx - \phi \\
        &= (z - ((\phi - \sigma )- n) )x - \phi \\
\end{align}

Therefore \(\dot{x} = (z-k)x - \phi\) for \(k = (\phi - \sigma) - n\) as
the problem asks for.

\begin{enumerate}
\def\labelenumi{\arabic{enumi}.}
\setcounter{enumi}{1}
\tightlist
\item
  \emph{Suppose policy aims to set \(z = \bar{z} > 0\) constant over
  time. What would happen to \(x\) over time if \(k>0\) and
  \(0<k<\bar{z}\)?}
\end{enumerate}

It's fairly easy to see that for \(\dot{x} = (z-k)x - \phi\) and
\((z-k)<0\) by assumption, then given our assumption that \(x,\phi > 0\)
it must be that \(\dot{x} < 0 \ \forall \ t\). Thus the ratio of the
human labor force (or human population as it were) to virulent mosquitos
goes down forever, presumably representing a sort of human extinction
event.

\hypertarget{task-b}{%
\subsection{Task B}\label{task-b}}

Disclaimer: The answer for several parts of this task admittedly go
\emph{much further} than requested in the question, in order to
drill-down into what all is happening behind the scenes with this
problem.

Now we are given \(c_t = \frac{C_t}{L_t}\) and told to imagine a planner
who wishes to maximize

\[U = \int^{\infty}_{0} e^{\rho t} u(c_t) dt\]

subject to the familiar state constraint

\[ \dot{x} = (z-k)x - \phi\]

\begin{enumerate}
\def\labelenumi{\arabic{enumi}.}
\tightlist
\item
  \emph{Using \(c = 1/b - \frac{az}{bx}\) and treating \(x\) as the
  state variable and \(z\) as the control, write down the Hamiltonian
  and the first-order conditions for an optimum.}
\end{enumerate}

\textbf{Answer:}

We are given the state to be \(z\) so the first order of business is to
substitute the given formula for \(c\) (which can even be derived from
the production possibilities frontier equation for given \(L\)) into the
utility function when we are forming the Hamiltonian:

\[ \mathcal{H_t} = u\left(\frac{1}{b} - \frac{a}{bx_t}z_t \right) + \lambda_t((z_t-k)x_t - \phi)\]

The first-order conditions for an optimum in this problem\footnote{Ignoring
  the second-derivative issue by assuming concavity of \(u(\cdot)\)} are
given by the following system of equations

\begin{align}

\frac{\partial u}{\partial c_t}\frac{\partial c_t}{\partial z_t} + \lambda_t x_t &= 0 \\

\dot{\lambda} = \rho \lambda_t - \frac{\partial \mathcal{H_t}}{\partial x_t} &= \rho \lambda_t - \left[\frac{\partial u}{\partial c_t}\frac{\partial c_t}{\partial x_t} + \lambda_t (z_t - k) \right] \\

\lim_{t \to \infty} e^{-\rho t}\lambda_t x_t &= 0 

\end{align}

One thing we'll need is \(\partial c_t/\partial z_t\) and
\(\partial c_t/\partial x_t\) to solve this. Let's also just call
\(u' \equiv \frac{\partial u}{\partial c_t}\)

\begin{align}

\frac{\partial c_t}{\partial z_t} &= -\frac{a}{bx_t} \\
\frac{\partial c_t}{\partial x_t} &= (-1)\left(-\frac{az_t}{bx_t^2}\right)  \\
&= \frac{\partial c_t}{\partial z_t}\left(-\frac{z_t}{x_t}\right)

\end{align}

With these, let's substitute and re-write the first-order conditions:

\begin{align}
\left( -\frac{a}{bx_t}\right)u' + \lambda_tx_t &= 0 \\
\Rightarrow \lambda_t = \frac{a}{bx_t^2}u' &= \frac{\partial c_t}{\partial x_t}\frac{u'}{z_t} \\
\dot{\lambda} = \rho \lambda_t - \left[ (\lambda_t z_t) + \lambda_t z_t - \lambda_t k \right] &= (\rho - 2z_t + k)\lambda_t \\
\Rightarrow \frac{\dot{\lambda}}{\lambda_t} &= \rho - 2z_t + k

\end{align}

Carefully note the substitution made for
\(u'\frac{\partial c_t}{\partial x_t}\) on the third line. To finish out
the model solution, all we need is a closed-form expression for
\(\dot{\lambda} \equiv \frac{d\lambda}{dt}\). For this particular model
where \(z_t\) is the control, this is about as painless as pulling your
own tooth, and so George doesn't ask for this on the actual exam. We
shall not be deterred so easily however. I'll mostly drop time
subscripts from here on out.

\begin{align}

\lambda_t = \frac{a}{b}\frac{u'(z_t , x_t)}{x_t^2} \Rightarrow \frac{d\lambda}{dt} &= \frac{a}{b}\left[\frac{(d/dt \ u')x_t^2 - (d/dt \ x_t^2)u'}{x_t^4}\right] \\
&= \frac{a}{b}\left[\frac{u''\cdot(\frac{\partial c}{\partial z}\dot{z} + \frac{\partial c}{\partial x}\dot{x})x_t^2 - 2u'x_t\dot{x}}{x_t^4} \right] \\ 
&= \frac{a}{bx_t^2}\left[\frac{u''\frac{\partial c}{\partial z}(\dot{z} - \frac{z}{x}\dot{x})x_t^2 - 2u'x_t\dot{x}}{x_t^2} \right] \\
\Rightarrow \frac{\dot{\lambda}}{\lambda} = \frac{\frac{a}{bx^2}(\frac{u''\partial c}{\partial z}(\dot{z} - \frac{z}{x}\dot{x})x_t^2 - 2x_tu'\dot{x})/x_t^2}{\frac{a}{bx^2}u'} &= \frac{\partial c}{\partial z}\frac{u''}{u'}(\dot{z} - \frac{z}{x}\dot{x}) - 2\frac{\dot{x}}{x}

\end{align}

And we have it-- an expression for \(\frac{\dot{\lambda}}{\lambda}\)
that we can substitute into the first-order condition:
\[ \frac{\dot{\lambda}}{\lambda} = \frac{a}{bx}\frac{u''}{u'}\left(z\frac{\dot{x}}{x} - \dot{z}\right) - 2\frac{\dot{x}}{x} \]

As we substitute this into the left-hand side of the first-order
condition derived earlier, we'll divide both sides of the FOC by \(z\).

\[\frac{a}{bx}\frac{u''}{u'}\left(\frac{\dot{x}}{x} - \frac{\dot{z}}{z}\right) - \frac{2}{z}\frac{\dot{x}}{x} = \frac{\rho + k}{z} - 2\]

It will be helpful here to substitute \(\dot{x} = (z-k)x - \phi\) at
this point.

\begin{align}

\frac{a}{bx}\frac{u''}{u'}\left[z - k - \frac{\phi}{x} - \frac{\dot{z}}{z}\right] - \frac{2}{z}\left[(z-k) - \frac{\phi}{x}\right] &= \frac{\rho}{z} + \frac{k}{z} - 2 \\
\Rightarrow \frac{a}{bx}\frac{u''}{u'}\left[ z - k - \left( \frac{\dot{z}}{z} + \frac{\phi}{x}\right) \right] + \frac{2 \phi}{zx} &= \frac{(\rho - k)}{z} \\
\Rightarrow \frac{a}{bx}\frac{u''}{u'}\left[ z - k - \frac{\dot{z}}{z} - \frac{\phi}{x} \right] &= \frac{(\rho - k) - 2\phi/x}{z} \\
\Rightarrow \frac{u''}{u'}\left[ z - k - \frac{\dot{z}}{z} - \frac{\phi}{x} \right] &= \frac{b}{a}\left[\frac{(\rho - k)x - 2\phi}{z}\right] \\
\Rightarrow z - k - \frac{\dot{z}}{z} - \frac{\phi}{x} &= \frac{b[(\rho - k ) - 2\phi]}{az\frac{u''}{u'}} \\
\Rightarrow \frac{\dot{z}}{z} &= z - \frac{\phi}{x} - k - \frac{b(\rho - k)}{a\frac{zu''}{xu'}} - \frac{2b\phi}{az\frac{u''}{u'}} \\
\Rightarrow \frac{\dot{z}}{z} &= z - \left( \frac{\phi}{x} + \frac{\phi}{x}2b\frac{xu'}{azu''} \right)- b(\rho - k)\frac{xu'}{azu''} - k

\end{align}

Now that we've set-up and even solved the Hamiltonian, let's turn to the
second part of this questuon before we totally close this part of the
model off.

\begin{enumerate}
\def\labelenumi{\arabic{enumi}.}
\setcounter{enumi}{1}
\tightlist
\item
  \emph{For suitable U it can be shown that the first order conditions
  imply} \[\frac{\dot{z}}{z} = z - (1+\xi)\phi x^{-1} - A\] \emph{for
  constants A and \(\xi>0\). (You are not asked to show this). Compute
  the slopes dz/dx for the two curves \(\dot{x} = 0\) and
  \(\dot{z} = 0\).}
\end{enumerate}

George ultimately gave us the biggest hint here; ``For suitable
U\ldots{}'' We very often see utility functions for which
\[\frac{cu''(c)}{u'(c)} = \frac{1}{s'}\] for a constant
\(s'\).\footnote{These are called ``constant relative risk aversion''
  utility functions.} This function will need to be similar, with slight
differences though. Given our equation derived from the production
possibilities frontier, \(\frac{az}{x} = (1-bc)\), we could posit that

\[ \frac{azu''}{xu'} = \frac{1}{s} = \text{constant}\]

This would be fulfilled, for instance, if \(u = c - \gamma c^2\) and
\(b = 2\gamma\). Regardless, if we take this to be fulfilled in a manner
similar to the hint in the question, then for \(\xi = 2bs\) and
\(A=b(\rho - k)s + k\) then sure enough,

\[\frac{\dot{z}}{z} = z - (1+\xi)\frac{\phi}{x} - A\]

Adopting this notation going forward, we can see from setting
\(\dot{x} = 0 = (z - k)x - \phi\) we'll have
\(\tilde{z}= \frac{\phi}{\tilde{x}} + k\) and then

\[ \left. \frac{dz}{dx} \right\rvert_{\dot{x} = 0} = -\frac{\phi}{x^2}\]

Likewise if we set \(\dot{z} = 0 = z(z - (1+\xi)\frac{\phi}{x} - A)\)
then we get \(\hat{z}= (1+\xi)\frac{\phi}{\hat{x}} + A\) and in that
case,

\[ \left. \frac{dz}{dx} \right\rvert_{\dot{z} = 0} = -(1+\xi)\frac{\phi}{x^2}\]

\end{document}
